Refactor Syntax.v

doc/coq/simple/Syntax.v
@@ -291,16 +291,20 @@ Proof.
 Qed.
 
 (** Dynamics *)
-Inductive dy_ctx {time : Type} :=
+Inductive dy_ctx T :=
   | dy_hole
-  | dy_binde (x : ID) (tx : time) (C : dy_ctx)
-  | dy_bindm (M : ID) (CM : dy_ctx) (C : dy_ctx)
+  | dy_binde (x : ID) (tx : T) (C : dy_ctx T)
+  | dy_bindm (M : ID) (CM : dy_ctx T) (C : dy_ctx T)
 .
+
+Arguments dy_hole {T}.
+Arguments dy_binde {T}.
+Arguments dy_bindm {T}.
 
 Notation "'[|' '|]'" := (dy_hole) (at level 99).
 
 (* Auxiliary operators *)
-Fixpoint addr_x {time : Type} (C : @dy_ctx time) (x : ID) :=
+Fixpoint addr_x {T} (C : dy_ctx T) (x : ID) :=
   match C with
   | [||] => None
   | dy_binde x' tx' C' =>
@@ -308,7 +312,7 @@ Fixpoint addr_x {time : Type} (C : @dy_ctx time) (x : ID) :=
   | dy_bindm _ _ C' => addr_x C' x
   end.
 
-Fixpoint ctx_M {time : Type} (C : @dy_ctx time) (M : ID) :=
+Fixpoint ctx_M {T} (C : dy_ctx T) (M : ID) :=
   match C with
   | [||] => None
   | dy_binde _ _ C' => ctx_M C' M
@@ -324,14 +328,14 @@ Fixpoint st_level (C : st_ctx) :=
   | st_bindm _ C' C'' => S (Nat.max (st_level C') (st_level C''))
   end.
 
-Fixpoint dy_level {T} (C : @dy_ctx T) :=
+Fixpoint dy_level {T} (C : dy_ctx T) :=
   match C with
   | [||] => 0
   | dy_binde _ _ C' => S (dy_level C')
   | dy_bindm _ C' C'' => S (Nat.max (dy_level C') (dy_level C''))
   end.
 
-Fixpoint dy_to_st {T} (C : @dy_ctx T) :=
+Fixpoint dy_to_st {T} (C : dy_ctx T) :=
   match C with
   | [||] => [[||]]
   | dy_binde x _ C' => st_binde x (dy_to_st C')
@@ -339,12 +343,12 @@ Fixpoint dy_to_st {T} (C : @dy_ctx T) :=
   end.
 
 Lemma st_dy_level_eq {T} :
-  forall (C : @dy_ctx T), dy_level C = st_level (dy_to_st C).
+  forall (C : dy_ctx T), dy_level C = st_level (dy_to_st C).
 Proof.
   induction C; simpl; eauto.
 Qed.
 
-Lemma mod_is_static_none : forall {T} (dC : @dy_ctx T) (M : ID),
+Lemma mod_is_static_none : forall {T} (dC : dy_ctx T) (M : ID),
   (ctx_M dC M = None <-> st_ctx_M (dy_to_st dC) M = None).
 Proof. 
   intros. repeat split; induction dC; simpl; eauto;
@@ -355,7 +359,7 @@ Proof.
   end.
 Qed.
 
-Lemma mod_is_static_some : forall {T} (dC : @dy_ctx T) (M : ID),
+Lemma mod_is_static_some : forall {T} (dC : dy_ctx T) (M : ID),
   (forall v, ctx_M dC M = Some v -> st_ctx_M (dy_to_st dC) M = Some (dy_to_st v)) /\
   (forall v, st_ctx_M (dy_to_st dC) M = Some v -> exists dv, dy_to_st dv = v /\ ctx_M dC M = Some dv).
 Proof.
@@ -373,374 +377,196 @@ Proof.
 Qed.
 
 (* More semantic domains *)
-Inductive expr_value {time : Type} :=
-  | Closure (x : ID) (e : tm) (C : @dy_ctx time)
+Inductive expr_value T :=
+  | Closure (x : ID) (e : tm) (C : dy_ctx T)
 .
 
-Inductive dy_value {time : Type} :=
-  | EVal (ev : @expr_value time)
-  | MVal (mv : @dy_ctx time)
+Arguments Closure {T}.
+
+Inductive dy_value T :=
+  | EVal (ev : expr_value T)
+  | MVal (mv : dy_ctx T)
 .
 
-Definition memory {T} := T -> option (@expr_value T).
+Arguments EVal {T}.
+Arguments MVal {T}.
 
-Definition amemory {T} := T -> list (@expr_value T).
+Definition memory T := T -> option (expr_value T).
 
-Inductive config {T} :=
-  | Cf (e : tm) (C : @dy_ctx T) (m : @memory T) (t : T)
-  | Rs (V : @dy_value T) (m : @memory T) (t : T)
+Definition amemory T := T -> list (expr_value T).
+
+Inductive config T :=
+  | Cf (e : tm) (C : dy_ctx T) (m : memory T) (t : T)
+  | Rs (V : dy_value T) (m : memory T) (t : T)
 .
 
-Inductive aconfig {T} :=
-  | ACf (e : tm) (abs_C : @dy_ctx T) (abs_m : @amemory T) (abs_t : T)
-  | ARs (abs_V : @dy_value T) (abs_m : @amemory T) (abs_t : T)
+Arguments Cf {T}.
+Arguments Rs {T}.
+
+Inductive aconfig T :=
+  | ACf (e : tm) (abs_C : dy_ctx T) (abs_m : amemory T) (abs_t : T)
+  | ARs (abs_V : dy_value T) (abs_m : amemory T) (abs_t : T)
 .
+
+Arguments ACf {T}.
+Arguments ARs {T}.
 
 (* Definitions for the (finite) supports *)
-Fixpoint supp_C {T} (C : @dy_ctx T) (t : T) :=
+Fixpoint supp_C {T} (C : dy_ctx T) (t : T) :=
   match C with
   | [||] => False
   | dy_binde _ t' C' => t = t' \/ supp_C C' t
   | dy_bindm _ C' C'' => supp_C C' t \/ supp_C C'' t
   end.
 
-Definition supp_v {T} (v : @expr_value T) :=
+Definition supp_v {T} (v : expr_value T) :=
   match v with
   | Closure _ _ C => supp_C C
   end.
 
-Definition supp_V {T} (V : @dy_value T) :=
+Definition supp_V {T} (V : dy_value T) :=
   match V with
   | EVal ev => supp_v ev
   | MVal mv => supp_C mv
   end.
 
-Definition supp_m {T} (m : memory) (t : T) :=
+Definition supp_m {T} (m : memory T) (t : T) :=
   exists addr v, m addr = Some v /\ (addr = t \/ supp_v v t).
 
-Definition supp_ρ {T} (ρ : config) (t : T) :=
+Definition supp_ρ {T} (ρ : config T) (t : T) :=
   match ρ with
   | Cf _ C m time => supp_C C t \/ supp_m m t \/ time = t
   | Rs V m time => supp_V V t \/ supp_m m t \/ time = t
   end.
 
-(** Observational equivalence *)
-Inductive path :=
+(** Graph isomorphism between (C, m) and (C', m') *)
+Inductive node T :=
+  | Ptr (t : T)
+  | Ctx (C : dy_ctx T)
+.
+
+Arguments Ptr {T}.
+Arguments Ctx {T}.
+
+Inductive path T :=
   | Pnil
-  | Pe (x : ID) (tl : path)
-  | Pm (M : ID) (tl : path)
+  | Px (x : ID) (ntx : node T) (tl : path T)
+  | PM (M : ID) (nCM : node T) (tl : path T)
+  | Pv (v : value) (nCv : node T) (tl : path T)
 .
 
-Inductive view {T} :=
-  | Ctx (C : @dy_ctx T)
-  | Opq (* cannot observe more *)
-.
+Arguments Pnil {T}.
+Arguments Px {T}.
+Arguments PM {T}.
+Arguments Pv {T}.
 
-Fixpoint observe {T}
-  (V : @dy_value T) (m : @memory T) (p : path) :=
+Fixpoint pmap {T T'} (f : node T -> node T') (p : path T) :=
   match p with
-  | Pnil =>
-    match V with
-    | EVal (Closure x e C) =>
-      (Ctx C, [v_fn x e])
-    | MVal C => (Ctx C, [])
-    end
-  | Pe x tl =>
-    match observe V m tl with
-    | (Ctx C, obs) =>
-      match addr_x C x with
-      | None => (Opq, obs)
-      | Some t =>
-        match m t with
-        | None => (Opq, obs)
-        | Some (Closure x e C) =>
-          (Ctx C, (v_fn x e) :: obs)
-        end
-      end
-    | (_, obs) => (Opq, obs)
-    end
-  | Pm M tl =>
-    match observe V m tl with
-    | (Ctx C, obs) =>
-      match ctx_M C M with
-      | None => (Opq, obs)
-      | Some C => (Ctx C, obs)
-      end
-    | (_, obs) => (Opq, obs)
-    end
+  | Pnil => Pnil
+  | Px x ntx tl => Px x (f ntx) (pmap f tl)
+  | PM M nCM tl => PM M (f nCM) (pmap f tl)
+  | Pv v nCv tl => Pv v (f nCv) (pmap f tl)
   end.
 
-Definition path_of_t {T}
-  (V : @dy_value T) (m : @memory T) (t : T) (p : path) (x : ID) :=
-  match observe V m p with
-  | (Ctx C, _) =>
-    match addr_x C x with
-    | Some addr => t = addr
-    | None => False
+Fixpoint valid_path {T}
+  (V : dy_value T) (m : memory T) (p : path T) :=
+  match p, V with
+  | Pnil, _ => True
+  | Px x (Ptr tx) tl, MVal mv =>
+    match addr_x mv x with
+    | Some t => 
+      tx = t /\ (exists ev, Some ev = m t /\ valid_path (EVal ev) m tl)
+    | _ => False
     end
-  | _ => False
+  | PM M (Ctx CM) tl, MVal mv =>
+    match ctx_M mv M with
+    | Some C =>
+      CM = C /\ valid_path (MVal CM) m tl
+    | _ => False
+    end
+  | Pv v (Ctx Cv) tl, EVal ev =>
+    match ev with
+    | Closure x e C =>
+      v = v_fn x e /\ Cv = C /\ valid_path (MVal C) m tl
+    end
+  | _, _ => False
   end.
 
 Definition equiv {T T'}
-  (V : @dy_value T) (m : @memory T) (V' : @dy_value T') (m' : @memory T') :=
-  forall p,
-    match observe V m p, observe V' m' p with
-    | (Ctx C, obs), (Ctx C', obs') =>
-      obs = obs' /\
-      forall x,
-        match addr_x C x, addr_x C' x with
-        | Some t, Some t' =>
-          forall p' x',
-            path_of_t V m t p' x' <-> path_of_t V' m' t' p' x'
-        | None, None => True
-        | _, _ => False
-        end
-    | (Opq, obs), (Opq, obs') => obs = obs'
-    | _, _ => False
-    end.
+  (V : dy_value T) (m : memory T) (V' : dy_value T') (m' : memory T') :=
+  exists f f', forall p p',
+    (valid_path V m p -> valid_path V' m' (pmap f p)) /\
+    (valid_path V' m' p' -> valid_path V m (pmap f' p')).
 
 Notation "'<|' V1 m1 '≃' V2 m2 '|>'" :=
   (equiv V1 m1 V2 m2)
   (at level 10, V1 at next level, m1 at next level, V2 at next level, m2 at next level).
 
-Fixpoint aobs_view {T : Type}
-  (V : @dy_value T) (m : @amemory T) (p : path) :=
-  match p with
-  | pnil =>
-    match V with
-    | EVal (Closure x e C) => [Ctx C]
-    | MVal C => [Ctx C]
+Fixpoint avalid_path {T}
+  (V : dy_value T) (m : amemory T) (p : path T) :=
+  match p, V with
+  | Pnil, _ => True
+  | Px x (Ptr tx) tl, MVal mv =>
+    match addr_x mv x with
+    | Some t => 
+      tx = t /\ (exists ev, In ev (m t) /\ avalid_path (EVal ev) m tl)
+    | _ => False
     end
-  | pe x tl =>
-    List.fold_left (fun acc single_view =>
-    let new_views := match single_view with
-    | Ctx C =>
-      match addr_x C x with
-      | None => [Opq]
-      | Some t =>
-        List.fold_left (fun acc v => 
-        let new_view := match v with
-        | Closure x e C => Ctx C
-        end in
-        new_view :: acc) (m t) [Opq]
-      end
-    | _ => [Opq]
-    end in
-    new_views ++ acc) (aobs_view V m tl) []
-  | pm M tl =>
-    List.fold_left (fun acc single_view =>
-    let new_view := match single_view with
-    | Ctx C =>
-      match ctx_M C M with
-      | None => Opq
-      | Some C => Ctx C
-      end
-    | _ => Opq
-    end in
-    new_view :: acc) (aobs_view V m tl) []
-  end.
-
-Definition aptr_of_t {T} `{Eq T}
-  (V : @dy_value T) (m : @amemory T) (t : T) (p : path) :=
-  Inb t (List.fold_left (fun acc single_view =>
-    match single_view with
-    | Ptr t => t :: acc
-    | _ => acc
-    end) (aobs_view V m p) []).
-
-Fixpoint aobserve {T : Type} 
-  (V : @dy_value T) (m : @amemory T) (p : path) :=
-  match p with
-  | pnil =>
-    match V with
-    | EVal (Closure x e C) =>
-      [(Ctx C, [v_fn x e])]
-    | MVal C => [(Ctx C, [])]
+  | PM M (Ctx CM) tl, MVal mv =>
+    match ctx_M mv M with
+    | Some C =>
+      CM = C /\ avalid_path (MVal CM) m tl
+    | _ => False
     end
-  | pe x tl =>
-    List.fold_left (fun acc single_trace =>
-    let new_traces := match single_trace with
-    | (Ctx C, obs) =>
-      match addr_x C x with
-      | None => [(Opq, obs)]
-      | Some t =>
-        List.fold_left (fun acc v =>
-          let new_trace := match v with
-          | Closure x e C =>
-            (Ctx C, (v_fn x e) :: obs)
-          end in
-          new_trace :: acc) (m t) [(Opq, obs)]
-      end
-    | (_, obs) => [(Opq, obs)]
-    end in
-    new_traces ++ acc) (aobserve V m tl) []
-  | pm M tl =>
-    List.fold_left (fun acc single_trace =>
-    let new_trace := match single_trace with
-    | (Ctx C, obs) =>
-      match ctx_M C M with
-      | None => (Opq, obs)
-      | Some C => (Ctx C, obs)
-      end
-    | (_, obs) => (Opq, obs)
-    end in
-    new_trace :: acc) (aobserve V m tl) []
+  | Pv v (Ctx Cv) tl, EVal ev =>
+    match ev with
+    | Closure x e C =>
+      v = v_fn x e /\ Cv = C /\ avalid_path (MVal C) m tl
+    end
+  | _, _ => False
   end.
-
-Lemma union_map_comm A B :
-  forall (l acc : list A) (f : A -> B) g g'
-    (RR : forall a x, map f (g a x) = g' (map f a) (f x)),
-  map f (fold_left g l acc) = fold_left g' (map f l) (map f acc).
-Proof.
-  induction l; intros; simpl; eauto.
-  rewrite <- RR.
-  apply IHl. eauto.
-Qed.
-
-Lemma fold_map_comm T A B :
-  forall (l : list T) (acc : list A) (f : A -> B) g g'
-    (RR : forall a x, map f (g a x) = g' (map f a) x),
-  map f (fold_left g l acc) = fold_left g' l (map f acc).
-Proof.
-  induction l; intros; simpl; eauto.
-  rewrite <- RR.
-  apply IHl. eauto.
-Qed.
-
-Lemma app_map_comm A B :
-  forall (l1 l2 : list A) (f : A -> B),
-    map f (l1 ++ l2) = map f l1 ++ map f l2.
-Proof.
-  induction l1; simpl; eauto.
-  intros. rewrite IHl1. eauto.
-Qed.
-
-Lemma cut_tail_app T :
-  forall (tl l l' : list T),
-    l ++ tl = l' ++ tl <-> l = l'.
-Proof.
-  assert (forall (ll : list T), ll ++ [] = ll) as RR.
-  { induction ll; simpl; eauto. rewrite IHll. eauto. }
-  assert (forall (ll ll' : list T) (t : T) (EQ : ll ++ [t] = ll' ++ [t]), ll = ll').
-  { 
-    induction ll; induction ll'; intros; simpl in *; eauto;
-    inversion EQ; subst;
-    match goal with
-    | [H : [] = _ ++ [?t] |- _] =>
-      assert (In t []) as contra;
-      try (rewrite H; rewrite in_app_iff; right; simpl; eauto);
-      inversion contra
-    | [H : _ ++ [?t] = [] |- _] =>
-      assert (In t []) as contra;
-      try (rewrite <- H; rewrite in_app_iff; right; simpl; eauto);
-      inversion contra
-    | [H : _ ++ [?t] = _ ++ [?t] |- _] =>
-      apply IHll in H; subst; eauto
-    end. 
-  }
-  induction tl.
-  - intros. rewrite RR. rewrite RR. eauto.
-  - intros.
-    replace (a :: tl) with ([a] ++ tl) by reflexivity.
-    rewrite app_assoc. rewrite app_assoc.
-    rewrite IHtl.
-    split; eauto.
-    intros; subst; eauto.
-Qed.
-
-Lemma eq_aobs_view {T} `{Eq T} :
-  forall V m p, List.map fst (aobserve V m p) = @aobs_view T V m p.
-Proof.
-  intros.
-  induction p; simpl;
-  repeat des_goal; simpl in *; clarify; eauto;
-  rewrite <- IHp; apply union_map_comm;
-  induction a; intros; simpl; repeat des_goal; eauto;
-  rewrite app_map_comm;
-  rewrite cut_tail_app;
-  replace [Opq] with (map fst [(@Opq T, l)]) by reflexivity;
-  apply fold_map_comm; intros;
-  match goal with
-  | [l : list _ |- _] => 
-    (* most recently introduced *) 
-    induction l; repeat des_goal; simpl
-  end; eauto.
-Qed.
-
-Definition AObserve {T : Type} 
-  (V : @dy_value T) (m : @amemory T) (p : path) :=
-  List.map snd (aobserve V m p).
 
 Definition aequiv {T T'}
-  (V : @dy_value T) (m : @amemory T) (V' : @dy_value T') (m' : @amemory T') :=
-  forall (p : path) (vl : list value),
-    In vl (AObserve V m p) <-> In vl (AObserve V' m' p).
+  (V : dy_value T) (m : amemory T) (V' : dy_value T') (m' : amemory T') :=
+  exists f f', forall p p',
+    (avalid_path V m p -> avalid_path V' m' (pmap f p)) /\
+    (avalid_path V' m' p' -> avalid_path V m (pmap f' p')).
 
 Notation "'<|' V1 m1 '≃#' V2 m2 '|>'" :=
   (aequiv V1 m1 V2 m2)
   (at level 10, V1 at next level, m1 at next level, V2 at next level, m2 at next level).
 
 (* Translation of timestamps *)
-Fixpoint trans_C {T T'} (α : T -> T') (C : @dy_ctx T) :=
+Fixpoint trans_C {T T'} (α : T -> T') (C : dy_ctx T) :=
   match C with
   | [||] => [||]
   | dy_binde x t C' => dy_binde x (α t) (trans_C α C')
   | dy_bindm M CM C' => dy_bindm M (trans_C α CM) (trans_C α C')
   end.
 
-Definition trans_v {T T'} (α : T -> T') (v : @expr_value T) :=
+Definition trans_v {T T'} (α : T -> T') (v : expr_value T) :=
   match v with
   | Closure x e C => Closure x e (trans_C α C)
   end.
 
-Definition trans_V {T T'} (α : T -> T') (V : @dy_value T) :=
+Definition trans_V {T T'} (α : T -> T') (V : dy_value T) :=
   match V with
   | EVal v => EVal (trans_v α v)
   | MVal C => MVal (trans_C α C)
   end.
 
-Definition trans_m {T T'} (α : T -> T') (m : @memory T) (m' : @memory T') :=
-  forall t' v',
-    (m' t' = Some v' <->
-      exists t v, trans_v α v = v' /\ α t = t' /\ m t = Some v)
-.
-
-Definition abstract_m {CT AT} (α : CT -> AT) (m : @memory CT) (am : @amemory AT) :=
+Definition trans_m {CT AT} (α : CT -> AT) (m : memory CT) (am : amemory AT) :=
   forall abs_t abs_v,
     (In abs_v (am abs_t) <->
       exists t v, trans_v α v = abs_v /\ α t = abs_t /\ m t = Some v)
 .
 
-Definition trans_am {AT AT'} (α : AT -> AT') (am : @amemory AT) (am' : @amemory AT') :=
-  forall abs_t' abs_v',
-    (In abs_v' (am' abs_t') <->
-      exists abs_t abs_v, trans_v α abs_v = abs_v' /\ α abs_t = abs_t' /\ In abs_v (am abs_t))
-.
-
-Definition trans_ρ {T T'} (α : T -> T') (ρ : @config T) (ρ' : @config T') :=
-  match ρ, ρ' with
-  | Cf e C m t, Cf e' C' m' t' =>
-    e = e' /\ trans_C α C = C' /\ trans_m α m m' /\ α t = t'
-  | Rs V m t, Rs V' m' t' =>
-    trans_V α V = V' /\ trans_m α m m' /\ α t = t'
-  | _, _ => False
-  end.
-
-Definition abstract_ρ {CT AT} (α : CT -> AT) (ρ : @config CT) (aρ : @aconfig AT) :=
+Definition trans_ρ {CT AT} (α : CT -> AT) (ρ : config CT) (aρ : aconfig AT) :=
   match ρ, aρ with
   | Cf e C m t, ACf e' C' m' t' =>
-    e = e' /\ trans_C α C = C' /\ abstract_m α m m' /\ α t = t'
+    e = e' /\ trans_C α C = C' /\ trans_m α m m' /\ α t = t'
   | Rs V m t, ARs V' m' t' =>
-    trans_V α V = V' /\ abstract_m α m m' /\ α t = t'
-  | _, _ => False
-  end.
-
-Definition trans_aρ {T T'} (α : T -> T') (aρ : @aconfig T) (aρ' : @aconfig T') :=
-  match aρ, aρ' with
-  | ACf e C m t, ACf e' C' m' t' =>
-    e = e' /\ trans_C α C = C' /\ trans_am α m m' /\ α t = t'
-  | ARs V m t, ARs V' m' t' =>
-    trans_V α V = V' /\ trans_am α m m' /\ α t = t'
+    trans_V α V = V' /\ trans_m α m m' /\ α t = t'
   | _, _ => False
   end.
 
@@ -750,12 +576,12 @@ Lemma trans_C_addr :
     addr_x (trans_C α C) x = 
       match (addr_x C x) with 
       | None => None 
-      | Some addr => Some (α addr) 
+      | Some addr => Some (α addr)
       end.
 Proof.
   induction C; eauto.
   intros. simpl.
-  destruct (eqb_ID x0 x); eauto.
+  des_goal; eauto.
 Qed.
 
 Lemma trans_C_ctx_M :
@@ -768,11 +594,11 @@ Proof.
   - inversion ACCESS.
   - rewrite <- TRANS. simpl. apply IHC; eauto.
   - rewrite <- TRANS. simpl.
-    destruct (eqb_ID M0 M); eauto.
+    des_goal; eauto.
     inversion ACCESS; eauto.
 Qed.
 
-Fixpoint eq_C {T} eqb (C1 C2 : @dy_ctx T) :=
+Fixpoint eq_C {T} eqb (C1 C2 : dy_ctx T) :=
   match C1, C2 with
   | [||], [||] => true
   | dy_binde x1 t1 C1', dy_binde x2 t2 C2' =>
@@ -783,31 +609,30 @@ Fixpoint eq_C {T} eqb (C1 C2 : @dy_ctx T) :=
   end.
 
 Lemma ctx_refl {T} eqb (t_refl : forall t, eqb t t = true) : 
-  forall (C : @dy_ctx T), eq_C eqb C C = true.
+  forall (C : dy_ctx T), eq_C eqb C C = true.
 Proof.
   induction C; simpl; try rewrite ID_refl; try rewrite t_refl;
   try rewrite IHC; try rewrite IHC1; try rewrite IHC2; eauto.
 Qed.
 
-Lemma eq_C_st_eq {T} eqb (C1 C2 : @dy_ctx T) :
+Lemma eq_C_st_eq {T} eqb (C1 C2 : dy_ctx T) :
   eq_C eqb C1 C2 = true -> dy_to_st C1 = dy_to_st C2.
 Proof.
   intros EQ. revert C2 EQ.
   induction C1; induction C2; intros; simpl; eauto; try (inversion EQ; fail);
-  simpl in EQ.
-  destruct (eqb_ID x x0) eqn:EQID; try (inversion EQ; fail);
-  destruct (eqb tx tx0) eqn:EQt; try (inversion EQ; fail);
-  destruct (eq_C eqb C1 C2) eqn:EQC; try (inversion EQ; fail).
-  rewrite IHC1 with (C2 := C2); eauto.
-  replace x0 with x; eauto. rewrite <- eqb_ID_eq; eauto.
-  destruct (eqb_ID M M0) eqn:EQID; try (inversion EQ; fail);
-  destruct (eq_C eqb C1_1 C2_1) eqn:EQC1; try (inversion EQ; fail);
-  destruct (eq_C eqb C1_2 C2_2) eqn:EQC2; try (inversion EQ; fail).
-  erewrite IHC1_1; eauto. erewrite IHC1_2; eauto.
-  replace M0 with M. eauto. rewrite <- eqb_ID_eq; eauto.
+  simpl in EQ; repeat des_hyp;
+  repeat match goal with
+  | [H : context [eq_C eqb _ _ = true -> _] |- _] =>
+    match goal with
+    | [RR : eq_C eqb _ _ = true |- _] =>
+      apply H in RR; rewrite RR
+    end
+  | [RR : eqb_ID _ _ = true |- _] =>
+    rewrite eqb_ID_eq in RR; rewrite RR
+  end; eauto.
 Qed.
 
-Lemma eq_C_level_eq {T} eqb (C1 C2 : @dy_ctx T) :
+Lemma eq_C_level_eq {T} eqb (C1 C2 : dy_ctx T) :
   eq_C eqb C1 C2 = true -> dy_level C1 = dy_level C2.
 Proof.
   intros EQ.
@@ -817,7 +642,7 @@ Qed.
 
 (* injection, deletion *)
 
-Fixpoint inject {T} (Cout Cin : @dy_ctx T) :=
+Fixpoint inject {T} (Cout Cin : dy_ctx T) :=
   match Cin with
   | [||] => Cout
   | dy_binde x t C' =>
@@ -826,7 +651,7 @@ Fixpoint inject {T} (Cout Cin : @dy_ctx T) :=
     dy_bindm M (inject Cout C') (inject Cout C'')
   end.
 
-Fixpoint delete {T} eqb (Cout Cin : @dy_ctx T) :=
+Fixpoint delete {T} eqb (Cout Cin : dy_ctx T) :=
   if eq_C eqb Cout Cin then [||]
   else match Cin with
   | [||] => [||]
@@ -836,49 +661,59 @@ Fixpoint delete {T} eqb (Cout Cin : @dy_ctx T) :=
     dy_bindm M (delete eqb Cout Cin') (delete eqb Cout Cin'')
   end.
 
-Lemma inject_level_inc {T} (Cout Cin : @dy_ctx T) :
+Lemma inject_level_inc {T} (Cout Cin : dy_ctx T) :
   dy_level Cout <= dy_level (inject Cout Cin).
 Proof.
   induction Cin; intros; simpl; nia.
 Qed.
 
 Lemma delete_inject_eq {T} eqb (t_refl : forall t, eqb t t = true) :
-  forall (Cout Cin : @dy_ctx T),
+  forall (Cout Cin : dy_ctx T),
     delete eqb Cout (inject Cout Cin) = Cin.
 Proof.
-  intros. revert Cout. induction Cin; simpl.
-  - induction Cout; eauto;
-    simpl; rewrite ID_refl; try rewrite t_refl; repeat rewrite ctx_refl; eauto.
-  - intros. rewrite IHCin.
-    destruct (eq_C eqb Cout (dy_binde x tx (inject Cout Cin))) eqn:F; eauto.
-    assert (dy_level Cout = dy_level (dy_binde x tx (inject Cout Cin))) as RR.
-    { eapply eq_C_level_eq; eauto. }
-    simpl in RR.
-    pose proof (inject_level_inc Cout Cin) as contra. nia.
-  - intros. rewrite IHCin1. rewrite IHCin2.
-    destruct (eq_C eqb Cout (dy_bindm M (inject Cout Cin1) (inject Cout Cin2))) eqn:F; eauto.
-    assert (dy_level Cout = dy_level (dy_bindm M (inject Cout Cin1) (inject Cout Cin2))) as RR.
-    { eapply eq_C_level_eq; eauto. }
-    simpl in RR.
-    pose proof (inject_level_inc Cout Cin1) as contra1.
-    pose proof (inject_level_inc Cout Cin2) as contra2. nia.
+  intros. revert Cout. induction Cin; simpl;
+  match goal with
+  | |- context [if _ then _ else _] =>
+    (* inductive case *)
+    intros; try rewrite IHCin; try rewrite IHCin1; try rewrite IHCin2;
+    des_goal; eauto;
+    (* search for a contradiction *)
+    match goal with
+    | [H : eq_C _ _ _ = true |- _] =>
+      apply eq_C_level_eq in H; simpl in H
+    end;
+    match goal with
+    | [H : dy_level ?Cout = _|-_] =>
+      match type of H with
+      | context [inject ?Cout ?Cin] =>
+        pose proof (inject_level_inc Cout Cin); try nia
+      end
+    end
+  | _ =>
+    (* base case *)
+    induction Cout; eauto;
+    simpl;
+    repeat rewrite ID_refl;
+    repeat rewrite t_refl;
+    repeat rewrite ctx_refl; eauto
+  end.
 Qed.
   
 Notation "Cin '[|' Cout '|]'" := (inject Cout Cin)
                               (at level 99, Cout at next level, right associativity).
 
-Definition inject_v {T} `{Eq T} (Cout : @dy_ctx T) (v : @expr_value T) :=
+Definition inject_v {T} `{Eq T} (Cout : dy_ctx T) (v : expr_value T) :=
   match v with
   | Closure x t C => Closure x t (Cout [|C|])
   end.
 
-Definition delete_v {T} eqb (Cout : @dy_ctx T) (v : @expr_value T) :=
+Definition delete_v {T} eqb (Cout : dy_ctx T) (v : expr_value T) :=
   match v with
   | Closure x t C => Closure x t (delete eqb Cout C)
   end.
 
 Lemma inject_ctx_M :
-  forall {T} `{Eq T} M (Cout Cin : @dy_ctx T),
+  forall {T} `{Eq T} M (Cout Cin : dy_ctx T),
     ctx_M (Cin [| Cout |]) M =
     match ctx_M Cin M with
     | Some CM => Some (CM [| Cout |])
@@ -888,11 +723,11 @@ Proof.
   intros. revert Cout.
   induction Cin; intros; simpl; eauto.
   rewrite IHCin2.
-  destruct (eqb_ID M M0); eauto.
+  des_goal; eauto.
 Qed.
 
 Lemma inject_addr_x :
-  forall {T} `{Eq T} x (Cout Cin : @dy_ctx T),
+  forall {T} `{Eq T} x (Cout Cin : dy_ctx T),
     addr_x (Cin [| Cout |]) x =
     match addr_x Cin x with
     | Some t => Some t
@@ -902,12 +737,12 @@ Proof.
   intros. revert Cout.
   induction Cin; intros; simpl; eauto.
   rewrite IHCin.
-  destruct (eqb_ID x x0); eauto.
+  des_goal; eauto.
 Qed.
 
 (* lemmas for trans_C *)
 Lemma trans_C_id_eq {T} :
-  forall (C : @dy_ctx T), trans_C id C = C.
+  forall (C : dy_ctx T), trans_C id C = C.
 Proof.
   induction C; simpl; try rewrite IHC; eauto.
   rewrite IHC1. rewrite IHC2. reflexivity.
@@ -918,24 +753,30 @@ Lemma eq_C_eq {T} `{Eq T} :
   eq_C eqb C C' = true <-> C = C'.
 Proof.
   induction C; destruct C'; simpl;
-  try (split; intros contra; inversion contra; eauto; fail).
-  - split; intros EQ.
-    + destruct (eqb_ID x x0) eqn:EQid; try (inversion EQ; fail);
-      destruct (eqb tx tx0) eqn:EQt; try (inversion EQ; fail).
-      simpl in EQ.
-      rewrite IHC in EQ. rewrite eqb_ID_eq in EQid. rewrite eqb_eq in EQt.
-      subst; eauto.
-    + inversion EQ. subst. rewrite ID_refl. rewrite t_refl. simpl.
-      apply IHC. eauto.
-  - split; intros EQ.
-    + destruct (eqb_ID M M0) eqn:EQid; try (inversion EQ; fail);
-      destruct (eq_C eqb C1 C'1) eqn:EQC1; try (inversion EQ; fail).
-      simpl in EQ.
-      rewrite IHC2 in EQ. rewrite eqb_ID_eq in EQid. rewrite IHC1 in EQC1.
-      subst; eauto.
-    + inversion EQ. subst. rewrite ID_refl. simpl.
-      replace (eq_C eqb C'1 C'1) with true. simpl.
-      apply IHC2. eauto. symmetry. apply IHC1. eauto.
+  try (split; intros contra; inversion contra; fail);
+  split; intros EQ;
+  repeat des_hyp; try reflexivity;
+  repeat match goal with
+  | [H : eqb_ID _ _ = true|-_] => rewrite eqb_ID_eq in H
+  | [H : eqb _ _ = true|-_] => rewrite eqb_eq in H
+  | [H : eq_C _ _ _ = true|-_] => 
+    try rewrite IHC in H;
+    try rewrite IHC1 in H;
+    try rewrite IHC2 in H
+  | _ => clarify
+  end; try reflexivity;
+  try rewrite ID_refl;
+  try rewrite t_refl;
+  repeat match goal with
+  | |- context[eq_C ?eqb ?C ?C] =>
+    match goal with
+    | [H : context [eq_C eqb C _ = true <-> _] |- _] =>
+      let RR := fresh "RR" in
+      assert (eq_C eqb C C = true) as RR;
+      try rewrite H; eauto; rewrite RR
+    end
+  | _ => idtac
+  end.
 Qed.
 
 Lemma trans_C_eq_C {CT AT} `{ECT : Eq CT} `{EAT : Eq AT} (α : CT -> AT) :
@@ -945,38 +786,33 @@ Lemma trans_C_eq_C {CT AT} `{ECT : Eq CT} `{EAT : Eq AT} (α : CT -> AT) :
     trans_C α C = trans_C α C'.
 Proof.
   induction C; induction C'; simpl;
-  try (split; intros contra; inversion contra; eauto; fail).
-  - split; intros EQ.
-    + destruct (eqb_ID x x0) eqn:EQid;
-      try (inversion EQ; fail).
-      destruct (eqb (α tx) (α tx0)) eqn:EQt;
-      try (inversion EQ; fail).
-      destruct (eq_C (fun t t' : CT => eqb (α t) (α t')) C C') eqn:EQC;
-      try (inversion EQ; fail).
-      rewrite eqb_ID_eq in EQid. rewrite eqb_eq in EQt.
-      specialize (IHC C').
-      rewrite EQid. rewrite EQt. 
-      replace (trans_C α C') with (trans_C α C). reflexivity. 
-      apply IHC. eauto.
-    + inversion EQ; subst. rewrite ID_refl. simpl.
-      rewrite t_refl. simpl.
-      rewrite IHC. eauto.
-  - split; intros EQ.
-    + destruct (eqb_ID M M0) eqn:EQid;
-      try (inversion EQ; fail).
-      destruct (eq_C (fun t t' : CT => eqb (α t) (α t')) C1 C'1) eqn:EQC1;
-      try (inversion EQ; fail).
-      destruct (eq_C (fun t t' : CT => eqb (α t) (α t')) C2 C'2) eqn:EQC2;
-      try (inversion EQ; fail).
-      rewrite eqb_ID_eq in EQid.
-      specialize (IHC1 C'1). specialize (IHC2 C'2).
-      rewrite EQid.
-      replace (trans_C α C'1) with (trans_C α C1).
-      replace (trans_C α C'2) with (trans_C α C2). reflexivity.
-      rewrite <- IHC2. eauto. rewrite <- IHC1. eauto.
-    + inversion EQ; subst. rewrite ID_refl. simpl.
-      replace (eq_C (fun t t' : CT => eqb (α t) (α t')) C1 C'1) with true. simpl.
-      rewrite IHC2. eauto. symmetry. rewrite IHC1. eauto.
+  try (split; intros contra; inversion contra; eauto; fail);
+  split; intros EQ;
+  repeat des_hyp;
+  repeat match goal with
+  | [H : eqb_ID _ _ = true|-_] => 
+    rewrite eqb_ID_eq in H; rewrite H
+  | [H : eqb _ _ = true|-_] => 
+    rewrite eqb_eq in H; rewrite H
+  | [H : eq_C _ _ _ = true|-_] => 
+    try rewrite IHC in H;
+    try rewrite IHC1 in H;
+    try rewrite IHC2 in H;
+    rewrite H
+  | _ => clarify
+  end; try reflexivity;
+  try rewrite ID_refl;
+  repeat match goal with
+  | [RR : α _ = α _|-_] => rewrite RR; rewrite t_refl
+  | |- context[eq_C ?eqb' ?C ?C'] =>
+    match goal with
+    | [H : context [eq_C _ C _ = true <-> _]|-_] =>
+      let RR := fresh "RR" in
+      assert (eq_C eqb' C C' = true) as RR;
+      try rewrite H; try assumption; rewrite RR
+    | _ => fail
+    end
+  end; eauto.
 Qed.
 
 Lemma trans_C_delete {CT AT} `{ECT : Eq CT} `{EAT : Eq AT} (α : CT -> AT) :
@@ -989,11 +825,9 @@ Proof.
   { induction Cout; induction C'; eauto.
     simpl. rewrite IHCout. eauto.
     simpl. rewrite IHCout1. rewrite IHCout2. eauto. }
-  induction C; intros; simpl; rewrite RR; simpl.
-  - destruct (eq_C eqb (trans_C α Cout) ([||])); eauto.
-  - destruct (eq_C eqb (trans_C α Cout) (dy_binde x (α tx) (trans_C α C))); eauto.
-    simpl. rewrite IHC. eauto.
-  - destruct (eq_C eqb (trans_C α Cout)
-      (dy_bindm M (trans_C α C1) (trans_C α C2))); eauto.
-    simpl. rewrite IHC1. rewrite IHC2. eauto.
+  induction C; intros; simpl; rewrite RR; simpl;
+  des_goal; eauto;
+  try rewrite IHC;
+  try rewrite IHC1;
+  try rewrite IHC2; eauto.
 Qed.
